Play with the idea of reifying "Valid" terms, but this is far too slow
We end up adding back in tons of typing information, in order to simplify the
proofs, but really the possibility of failure is OK, is just means there are
solvable things that the tactic might not solve. I'm committing this just for
archival purposes, but will rip out the new code shortly.

src/Solver.v
@@ -318,11 +318,31 @@ Fixpoint denote dom cod (e : Term) :
 
 (* Define what it means for a Term to be valid within a given context. *)
 Fixpoint Valid dom cod (e : Term) : Type :=
+  TermDom e = dom ∧
+  TermCod e = cod ∧
   match e with
   | Identity x  => dom = cod ∧ dom = x
   | Morph x y f => dom = x ∧ cod = y ∧ ∃ f', arrs f x y = Some f'
   | Compose f g => Valid (TermCod g) cod f ∧ Valid dom (TermCod g) g
   end.
+
+Ltac equalities :=
+  repeat match goal with
+    | [ H : (_ &&& _) = true |- _ ] =>
+      rewrite <- andb_lazy_alt in H
+    | [ H : (_ && _) = true |- _ ] =>
+      apply andb_true_iff in H;
+      destruct H
+    | [ H : _ /\ _ |- _ ] =>
+      destruct H
+    | [ H : _ ∧ _ |- _ ] =>
+      destruct H
+    | [ H : (_ =? _) = true |- _ ] =>
+      apply N.eqb_eq in H
+    end;
+  simpl TermDom in *;
+  simpl TermCod in *;
+  subst.
 
 (* Valid terms are easily denoted. *)
 Definition denote_valid dom cod :
@@ -334,12 +354,113 @@ Proof.
   generalize dependent cod.
   induction x; simpl; intros.
   - destruct v; subst.
+    equalities.
     exact id.
-  - destruct v, p, s; subst.
+  - equalities.
+    destruct s.
     exact x.
-  - destruct v.
+  - equalities.
     exact (IHx1 _ _ v ∘ IHx2 _ _ v0).
 Defined.
+
+Program Fixpoint mkComposeValid x y z (a b : Term) :
+  Valid y z a -> Valid x y b -> ∃ t : Term, Valid x z t := fun Ha Hb =>
+  match a with
+  | Identity _ => (b; Hb)
+  | _ => match b with
+        | Identity _  => (a; Ha)
+        | Compose g h => (Compose (Compose a g) h; _)
+        | _ => (Compose a b; (_, (_, (Ha, Hb))))
+        end
+  end.
+Next Obligation.
+  subst; simpl in *.
+  now equalities.
+Defined.
+Next Obligation.
+  subst; simpl in *.
+  now equalities.
+Defined.
+Next Obligation.
+  subst; simpl in *.
+  equalities; intuition.
+  - destruct a; simpl in *; now equalities.
+  - destruct g; simpl in *; now equalities.
+  - destruct a; simpl in *; now equalities.
+Defined.
+Next Obligation.
+  subst; simpl in *.
+  destruct b; simpl in *; now equalities.
+Defined.
+Next Obligation.
+  subst; simpl in *.
+  destruct a; simpl in *; now equalities.
+Defined.
+Next Obligation.
+  subst; simpl in *.
+  destruct b; simpl in *; now equalities.
+Defined.
+Next Obligation.
+  subst; simpl in *.
+  destruct b; simpl in *; now equalities.
+Defined.
+Next Obligation.
+  subst; simpl in *.
+  destruct b; simpl in *; now equalities.
+Defined.
+
+Definition normalizeValid dom cod (p : Term) :
+  Valid dom cod p -> ∃ t : Term, Valid dom cod t.
+Proof.
+  intros.
+  generalize dependent dom.
+  generalize dependent cod.
+  induction p; intros; simpl in X.
+  - exact (Identity n; X).
+  - exact (Morph n n0 n1; X).
+  - equalities.
+    destruct (IHp1 _ _ v)  as [f Hf].
+    destruct (IHp2 _ _ v0) as [g Hg].
+    exact (mkComposeValid _ (TermCod p2) _ f g Hf Hg).
+Defined.
+
+Theorem normalizeValid_sound_eq
+: ∀ p dom cod (H : Valid dom cod p) pV,
+    denote_valid dom cod (p; H) = pV ->
+    ∃ pV', pV ≈ pV' ∧ denote_valid dom cod (normalizeValid dom cod p H) = pV'.
+Proof.
+  induction p; intros.
+  - exists pV.
+    split; [reflexivity|].
+    simpl normalizeValid.
+    assumption.
+  - exists pV.
+    split; [reflexivity|].
+    simpl normalizeValid.
+    assumption.
+  - simpl in H.
+    equalities.
+    specialize (IHp1 (TermCod p2) _ v).
+    specialize (IHp2 _ (TermCod p2) v0).
+    destruct (IHp1 _ eq_refl).
+    destruct (IHp2 _ eq_refl).
+    equalities.
+Admitted.
+
+Theorem normalizeValid_apply dom cod : ∀ f g,
+  `1 (normalizeValid dom cod (`1 f) (`2 f)) =
+  `1 (normalizeValid dom cod (`1 g) (`2 g)) ->
+  denote_valid dom cod f ≈ denote_valid dom cod g.
+Proof.
+  generalize dependent dom.
+  generalize dependent cod.
+  intros.
+  destruct f, g; simpl in H.
+  generalize dependent dom.
+  generalize dependent cod.
+  generalize dependent x0.
+  induction x; intros.
+Admitted.
 
 End denote.
 
@@ -1152,6 +1273,35 @@ Ltac reifyTerm fs xs t :=
     end
   end.
 
+Ltac reifyValidTerm fs xs t objs arrs :=
+  match t with
+  | @id _ ?X =>
+    let x := lookup X xs in
+    constr:(existT (Valid _ objs arrs x x)
+                   (Identity x) (eq_refl, (eq_refl, (eq_refl, eq_refl))))
+  | ?X1 ∘ ?X2 =>
+    let r1 := reifyValidTerm fs xs X1 objs arrs in
+    match r1 with
+      (?r1_1; ?r1_2) =>
+      let r2 := reifyValidTerm fs xs X2 objs arrs in
+      match r2 with
+        (?r2_1; ?r2_2) =>
+        constr:(existT (Valid _ objs arrs (TermDom r2_1) (TermCod r1_1))
+                       (Compose r1_1 r2_1)
+                       (eq_refl, (eq_refl, (r1_2, r2_2))))
+      end
+    end
+  | ?F =>
+    let n := lookup F fs in
+    match type of F with
+    | ?X ~> ?Y =>
+      let x := lookup X xs in
+      let y := lookup Y xs in
+      constr:(existT (Valid _ objs arrs x y) (Morph x y n)
+                     (eq_refl, (eq_refl, (eq_refl, (eq_refl, (F; eq_refl))))))
+    end
+  end.
+
 Ltac objects_function xs :=
   let rec loop n xs' :=
     match xs' with
@@ -1182,6 +1332,8 @@ Ltac observe n f xs objs k :=
 Ltac arrows_function fs xs objs :=
   let rec loop n fs' :=
     match fs' with
+    | tt =>
+      constr:(fun _ x y : N => @None (objs x ~> objs y))
     | (?f, tt) =>
       observe n f xs objs (fun _ x y : N => @None (objs x ~> objs y))
     | (?f, ?fs'') =>
@@ -1201,27 +1353,36 @@ Ltac categorical :=
         (?fs, ?xs) =>
         pose xs;
         pose fs;
-        let r1  := reifyTerm fs xs S in
-        let r2  := reifyTerm fs xs T in
-        pose r1;
-        pose r2;
         let objs := objects_function xs in
         let arrs := arrows_function fs xs objs in
         pose objs;
         pose arrs;
-        change (denote _ objs arrs (TermDom r1) (TermCod r1) r1 ≈
-                denote _ objs arrs (TermDom r2) (TermCod r2) r2);
-        (* apply (normalize_apply_eq _ objs arrs (TermDom r1) (TermCod r1) *)
+        let r1  := reifyTerm fs xs S in
+        let r2  := reifyTerm fs xs T in
+        pose r1;
+        pose r2;
+        let r1'  := reifyValidTerm fs xs S objs arrs in
+        let r2'  := reifyValidTerm fs xs T objs arrs in
+        pose r1';
+        pose r2';
+        change (denote_valid _ objs arrs (TermDom (`1 r1')) (TermCod (`1 r1')) r1' ≈
+                denote_valid _ objs arrs (TermDom (`1 r2')) (TermCod (`1 r2')) r2');
+        apply (normalizeValid_apply
+                 _ objs arrs (TermDom (`1 r1')) (TermCod (`1 r1'))
+                 r1' r2')(* ; *)
+        (* change (denote _ objs arrs (TermDom r1) (TermCod r1) r1 ≈ *)
+        (*         denote _ objs arrs (TermDom r2) (TermCod r2) r2); *)
+        (* (* apply (normalize_apply_eq _ objs arrs (TermDom r1) (TermCod r1) *) *)
+        (* (*                        r1 (normalize r1) r2 (normalize r2) *) *)
+        (* (*                        eq_refl eq_refl); *) *)
+        (* apply (normalize_apply _ objs arrs (TermDom r1) (TermCod r1) *)
         (*                        r1 (normalize r1) r2 (normalize r2) *)
         (*                        eq_refl eq_refl); *)
-        apply (normalize_apply _ objs arrs (TermDom r1) (TermCod r1)
-                               r1 (normalize r1) r2 (normalize r2)
-                               eq_refl eq_refl);
-        simpl N.succ;
-        simpl normalize;
-        apply (@decision_correct _ objs arrs);
-        vm_compute;
-        auto
+        (* simpl N.succ; *)
+        (* simpl normalize; *)
+        (* apply (@decision_correct _ objs arrs); *)
+        (* vm_compute; *)
+        (* auto *)
       end
     end
   end.
@@ -1231,7 +1392,9 @@ Example sample_1 :
     f ∘ (id ∘ g ∘ h) ≈ (f ∘ g) ∘ h.
 Proof.
   intros.
-  categorical.
+  Time categorical.
+  vm_compute.
+  reflexivity.
 Qed.
 
 Print Assumptions sample_1.
